##### 2.

$$
T(n) = T(n-1) + n
\\\qquad \qquad \qquad =T(n-2) + n-1 + n
\\\qquad \qquad \qquad ...
\\\qquad \qquad \qquad \qquad \qquad =T(0) + 1 + 2 + ... + n-1 + n
\\\qquad \le T(0) + n^2
\\\quad = 1 + n^2
\\\quad = O(n^2)
$$

##### 4.

$$
T(n) = T({n \over 2}) + 1
\\\qquad\qquad = T({n \over 4}) + 1 + 1
\\\qquad\qquad ...
\\\qquad\qquad = T({n \over 2^k}) + k
\\\qquad n=2^k 대입 \rightarrow T(1) + \log n
\\\qquad = 1 + \log n
\\\qquad = O(\log n)
$$

##### 6.

$$
T(n) = 2\ T({n \over 2}) + n
\\\qquad\qquad = 4T({n \over 4}) + n + n
\\\qquad\qquad ...
\\\qquad\qquad\qquad\qquad\qquad = 2^kT({n \over 2^k}) + n+\ ...\ +n + n
\\\qquad\qquad = 2^kT({n \over 2^k}) + kn
\\ n=2^k 대입 \rightarrow nT(1) + n\log n
\\\qquad\qquad = n(T(1) + \log n)
\\\qquad = O(n\log n)
$$

##### 8.

$$
T(n) = T(n-1) + {1 \over n}
\\\qquad\qquad\qquad = T(n-2) + {1 \over n-1} + {1 \over n}
\\\qquad\qquad ...
\\\qquad\qquad\qquad\qquad = T(0) + 1 + {1 \over 2} +\ ...\ + {1 \over n}
\\\qquad\le T(0) + n
\\= O(n)
$$

